RewriteRules.v
@@ -1,9 +1,14 @@
 Require Import Eqdep Lists.List Lists.ListSet Vector Arith.PeanoNat Syntax AbstractRelation Bool.Sumbool Tribool 
-  Semantics JMeq FunctionalExtensionality Omega Coq.Init.Specif Translation2V ProofIrrelevance.
+  Semantics JMeq FunctionalExtensionality Omega Coq.Init.Specif ProofIrrelevance Util RelFacts SemFacts.
 
 Module RewriteRules (Db : DB) (Sql : SQL Db).
   Import Db.
   Import Sql.
+
+  Module RF := RelFacts.Facts Db Sql.
+  Module SF := SemFacts.Facts Db Sql.
+  Import RF.
+  Import SF.
 
   Module S2 := Sem2 Db.
   Module S3 := Sem3 Db.
@@ -22,113 +27,6 @@ Module RewriteRules (Db : DB) (Sql : SQL Db).
     + rewrite Rel.p_self; auto. destruct (Rel.memb S t) eqn:eSt; auto.
       erewrite H in ept. discriminate ept.
       apply Rel.p_fs. rewrite eSt. omega.
-  Qed.
-
-(*
-  Lemma cast_id A p a : cast A A p a = cast A A eq_refl a.
-  Proof.
-    rewrite (UIP_refl _ _ p).
-*)
-
-(*** XXX: currently in Translation2V, needs to be shared (e.g. in Facts.v) ***)
-Axiom list_sum_ext: forall Hdec l1,
-    forall l2, (forall x, count_occ Hdec l1 x = count_occ Hdec l2 x) ->
-    list_sum l1 = list_sum l2.
-Axiom eq_memb_dep : forall m n (e : m = n), forall (S1 : Rel.R m) (S2 : Rel.R n) r1 r2,
-  S1 ~= S2 -> r1 ~= r2 -> Rel.memb S1 r1 = Rel.memb S2 r2.
-Axiom eq_times_dep : forall m1 m2 n1 n2 (e1 : m1 = n1) (e2 : m2 = n2), 
-  forall (R1 : Rel.R m1) (R2 : Rel.R m2) (S1 : Rel.R n1) (S2 : Rel.R n2),
-  R1 ~= S1 -> R2 ~= S2 -> Rel.times R1 R2 ~= Rel.times S1 S2.
-Axiom p_ext_dep : forall m n (e : m = n), forall (S1 : Rel.R m) (S2 : Rel.R n),
-  (forall r1 r2, r1 ~= r2 -> Rel.memb S1 r1 = Rel.memb S2 r2) -> S1 ~= S2.
-
-Axiom daemon : forall (P : Prop), P.
-
-  Lemma cast_fun_app_JM A B A' B' B'' (ea : A = A') (eb : B = B') (eb' : B' = B'') :
-    forall (e : (A -> B) = (A' -> B')) (f : A -> B) (x : A') (y : B''), 
-    (forall x', x ~= x' -> f x' ~= y)
-    -> cast _ _ e f x ~= y.
-  Proof.
-    rewrite ea, eb, eb'. intro e. rewrite (UIP_refl _ _ e). intros. simpl.
-    apply H. reflexivity.
-  Qed.
-
-  Lemma JMeq_eq_rect A x (T : A -> Type) U t y e (u : U) : T y = U -> t ~= u -> eq_rect x T t y e ~= u.
-  Proof.
-    intros. generalize dependent t. rewrite e. simpl. intuition.
-  Qed.
-
-  Lemma JMeq_eq_rect_r A x (T : A -> Type) U t y e (u : U) : T y = U -> t ~= u -> @eq_rect_r _ x T t y e ~= u.
-  Proof.
-    intros. generalize dependent t. rewrite e. simpl. intuition.
-  Qed.
-
-  Lemma f_JMequal {A : Type} {B : A -> Type} {A' : Type} {B' : A' -> Type} 
-    {ea : A = A'} {eb : B ~= B'} :
-    forall (f : forall a, B a) (g : forall a', B' a') x y, f ~= g -> x ~= y -> f x ~= g y.
-  Proof.
-    generalize dependent eb. generalize dependent B'.
-    rewrite <- ea. intros B' eb.
-    eapply (eq_rect B (fun (B0 : A -> Type) =>
-      forall (f : forall a : A, B a) (g : forall a' : A, B0 a') (x y : A), f ~= g -> x ~= y -> f x ~= g y) _ B' _).
-    Unshelve.
-    simpl. intros. rewrite H, H0. reflexivity.
-    apply JMeq_eq. exact eb.
-  Qed.
-
-  Lemma f_JMequal_pi {A : Prop} {B : A -> Type} {A' : Prop} {B' : A' -> Type} 
-    {ea : A = A'} {eb : B ~= B'} :
-    forall (f : forall a, B a) (g : forall a', B' a') x y, f ~= g -> f x ~= g y.
-  (** not a corollary of the previous lemma, because here A = A' is (@eq Prop A A') rather than (@eq Type A A') *)
-  Proof.
-    generalize dependent eb. generalize dependent B'.
-    rewrite <- ea. intros B' eb.
-    eapply (eq_rect B (fun (B0 : A -> Type) =>
-      forall (f : forall a : A, B a) (g : forall a' : A, B0 a') (x y : A), f ~= g -> f x ~= g y) _ B' _).
-    Unshelve.
-    simpl. intros. rewrite H. rewrite (proof_irrelevance _ x y). reflexivity.
-    apply JMeq_eq. exact eb.
-  Qed.
-
-  Lemma f_JMeq : forall A (T : A -> Type) (f : forall a, T a) x y, x = y -> f x ~= f y.
-  Proof.
-    intros. rewrite H. reflexivity.
-  Qed.
-
-  Lemma existT_projT2_eq {A} {P : A -> Type} a (p1 p2 :  P a) (e : existT _ _ p1 = existT _ _ p2)
-    : p1 = p2.
-  Proof.
-    transitivity (projT2 (existT P a p1)). reflexivity. 
-    transitivity (projT2 (existT P a p2)). apply JMeq_eq. eapply (f_JMeq _ _ (@projT2 A P) _ _ e).
-    reflexivity.
-  Qed.
-
-  Lemma existT_eq_elim {A} {P : A -> Type} {a} {b} {p1} {p2} (e : existT P a p1 = existT P b p2) :
-    forall (Q:Prop), (a = b -> p1 ~= p2 -> Q) -> Q.
-  Proof.
-    intros. injection e. intros _ H1. generalize dependent p2. generalize dependent p1. 
-    rewrite H1. intros. apply H; auto. apply eq_JMeq. apply (existT_projT2_eq _ _ _ e).
-  Qed.
-
-  Lemma cast_JMeq S T U e x (y : U) : x ~= y -> cast S T e x ~= y.
-  Proof.
-    generalize dependent x. rewrite e. simpl. intuition.
-  Qed.
-
-  Lemma cast_elim {P:Prop} {A} (B : Type) (a : A) : A = B -> (forall (b:B), a ~= b -> P) -> P.
-  Proof.
-    intros; subst. apply (H0 _ JMeq_refl).
-  Qed.
-
-  Lemma vector_append_nil_r {A} {n} (v : Vector.t A n): 
-    append v (Vector.nil _) ~= v.
-  Proof.
-    induction v; intuition.
-    simpl. eapply (f_JMequal (cons A h (n+0)) (cons A h n)). Unshelve.
-    + eapply (f_JMeq _ _ (cons A h)). omega.
-    + exact IHv.
-    + f_equal. omega.
-    + replace (n+0) with n. reflexivity. omega.
   Qed.
 
 (*
@@ -232,243 +130,6 @@ Axiom daemon : forall (P : Prop), P.
         * rewrite H10, H13. reflexivity.
   Qed.
 
-  Lemma tech_commutative_join A B (l1 : list A) (l2 : list B) f g h :
-    (forall x, count_occ Nat.eq_dec (List.map f l1) x = count_occ Nat.eq_dec (List.map g (List.map h l1)) x) ->
-    (forall x, count_occ Nat.eq_dec (List.map g (List.map h l1)) x = count_occ Nat.eq_dec (List.map g l2) x) ->
-    forall x, count_occ Nat.eq_dec (List.map f l1) x = count_occ Nat.eq_dec (List.map g l2) x.
-  Proof.
-    intuition. etransitivity. apply H. apply H0.
-  Qed.
-
-  Axiom tech2_commutative_join : forall A B C (l : list A) (f : A -> C) (g : B -> C) (h : A -> B),
-    (forall x, f x = g (h x)) ->
-    List.map f l = List.map g (List.map h l).
-
-  Axiom tech3_commutative_join : forall A B Hdec g (h : A -> B) l1 l2,
-    (forall x, count_occ Hdec (List.map h l1) x = count_occ Hdec l2 x) ->
-    forall x, count_occ Nat.eq_dec (List.map g (List.map h l1)) x = count_occ Nat.eq_dec (List.map g l2) x.
-
-  Axiom tech4_commutative_join : forall A B HdecA HdecB (h : A -> B) p1 p2 l1 l2,
-    (forall x, count_occ HdecA l1 x = count_occ HdecB l2 (h x) /\ p1 x = p2 (h x)) ->
-    forall x, count_occ HdecB (List.map h (List.filter p1 l1)) x = count_occ HdecB (List.filter p2 l2) x.
-
-  (** XXX: copied from Semantics **)
-  (* naturally splits a Vector of size (m+n) into two Vectors of sizes m and n *)
-  Fixpoint split {A} {m} {n} : Vector.t A (m+n) -> (Vector.t A m * Vector.t A n).
-  refine
-  (match m as m return Vector.t A (m+n) -> (Vector.t A m * Vector.t A n) with
-   | 0 => fun v => (nil _,v)
-   | S p => fun v => let h := Vector.hd v in let t := Vector.tl v in
-      let (v1,v2) := split _ _ _ t in
-      (Vector.cons _ h _ v1,v2)
-   end).
-  Defined.
-
-  Definition flip {A} {m} {n} : Vector.t A (m + n) -> Vector.t A (n + m) :=
-    fun v => let (v1,v2) := split v in Vector.append v2 v1.
-
-  Lemma eq_T_eqb_iff {m} {n} (t1 t2 : Rel.T m) (t3 t4 : Rel.T n) : 
-    (t1 = t2 <-> t3 = t4) -> Rel.T_eqb t1 t2 = Rel.T_eqb t3 t4.
-  Proof.
-    destruct (Rel.T_eqb t1 t2) eqn:e1; destruct (Rel.T_eqb t3 t4) eqn:e2; intuition; auto.
-    + rewrite <- e2. symmetry. apply Rel.T_eqb_eq. apply H0. apply Rel.T_eqb_eq. exact e1.
-    + rewrite <- e1. apply Rel.T_eqb_eq. apply H1. apply Rel.T_eqb_eq. exact e2.
-  Qed.
-
-  Lemma cast_fun_app A B A' B' (ea : A = A') (eb : B = B') :
-    forall (e : (A -> B) = (A' -> B')) (f : A -> B) (x : A') (y : B'), 
-    (forall x', x ~= x' -> f x' ~= y)
-    -> cast _ _ e f x = y.
-  Proof.
-    rewrite ea, eb. intro e. rewrite (UIP_refl _ _ e). intros. simpl.
-    apply JMeq_eq. apply H. reflexivity.
-  Qed.
-
-  Lemma split_0_l {A} {n} (v : Vector.t A (0 + n)) :
-    forall (v0 : Vector.t A n), v ~= v0 <-> split v = (Vector.nil _, v0).
-  Proof.
-    simpl. intuition.
-    + rewrite H; reflexivity.
-    + injection H; intuition; rewrite H0; reflexivity.
-  Qed.
-
-  Lemma hd_equal {A} {m} {n} (v1 : Vector.t A (S m)) (v2 : Vector.t A (S n)) :
-    m = n -> v1 ~= v2 -> hd v1 = hd v2.
-  Proof.
-    intro. subst. intro. rewrite H. reflexivity.
-  Qed.
-
-  Lemma tl_equal {A} {m} {n} (v1 : Vector.t A (S m)) (v2 : Vector.t A (S n)) :
-    m = n -> v1 ~= v2 -> tl v1 ~= tl v2.
-  Proof.
-    intro. subst. intro. rewrite H. reflexivity.
-  Qed.
-
-  Lemma cons_equal {A} : forall h1 h2 n1 n2 t1 t2,
-    h1 = h2 -> n1 = n2 -> t1 ~= t2 -> cons A h1 n1 t1 ~= cons A h2 n2 t2.
-  Proof.
-    intros. generalize t1 t2 H1; clear t1 t2 H1. rewrite H, H0.
-    intros. rewrite H1. reflexivity.
-  Qed.
-
-  Lemma fst_split_0_r {A} {n} (v : Vector.t A (n + 0)) : fst (split v) ~= v.
-  Proof.
-    generalize dependent v. induction n; simpl.
-    + intro. eapply (case0 _ _ v). Unshelve. reflexivity.
-    + intros. eapply (caseS' v). simpl. intros.
-      replace (split t) with (fst (split t), snd (split t)). simpl.
-      apply cons_equal. reflexivity. omega. apply IHn.
-      rewrite surjective_pairing. reflexivity.
-  Qed.
-
-  Lemma split_ind {A} {m} {n} (v : Vector.t A (m + n)) :
-    forall (P : forall m n, (Vector.t A m * Vector.t A n) -> Prop),
-    (forall v1 v2, v = append v1 v2 -> P m n (v1,v2)) ->
-    P m n (split v).
-  Proof.
-    induction m; simpl; intuition.
-    rewrite (surjective_pairing (split (tl v))). apply H. apply JMeq_eq.
-    eapply (IHm (tl v) (fun m0 n0 v0 => v ~= append (cons A (hd v) _ (fst v0)) (snd v0))).
-    intros. simpl. rewrite (Vector.eta v). simpl. apply eq_JMeq. f_equal. exact H0.
-  Qed.
-
-  Lemma split_0_r {A} {n} (v : Vector.t A (n + 0)) :
-    forall (v0 : Vector.t A n), v ~= v0 <-> split v = (v0, Vector.nil _).
-  Proof.
-    induction n; simpl; intuition.
-    + f_equal. eapply (case0 _ _ v0). eapply (case0 (fun v => v = nil A) _ v). Unshelve.
-      reflexivity. reflexivity.
-    + injection H. intuition. subst. reflexivity.
-    + generalize dependent H. apply (caseS' v). apply (caseS' v0).
-      intuition. simpl. destruct (IHn t0 t). rewrite H0.
-      f_equal. f_equal. 
-      enough (hd (cons A h0 (n+0) t0) = hd (cons A h n t)). exact H2. apply hd_equal.
-      omega. exact H.
-      enough (tl (cons A h0 (n+0) t0) ~= tl (cons A h n t)). exact H2. apply tl_equal.
-      omega. exact H.
-    + generalize dependent H. apply (caseS' v). apply (caseS' v0).
-      intuition. simpl in H. replace (split t0) with (fst (split t0), snd (split t0)) in H.
-      enough (fst (cons A h0 n (fst (split t0)), snd (split t0)) ~= fst (cons A h n t, nil A)).
-      simpl in H0. rewrite <- H0. apply cons_equal. reflexivity. apply plus_0_r. symmetry. apply fst_split_0_r.
-      rewrite H. reflexivity. rewrite surjective_pairing. reflexivity.
-  Qed.
-
-  Lemma vec_append_inj {A} {m} {n} {v1 v2 : Vector.t A m} {v3 v4 : Vector.t A n}
-    : append v1 v3 = append v2 v4 -> v1 = v2 /\ v3 = v4.
-  Proof.
-    induction m; simpl.
-    + eapply (case0 (fun v0 => append v0 v3 = append v2 v4 -> v0 = v2 /\ v3 = v4)).
-      eapply (case0 (fun v0 => append (nil A) v3 = append v0 v4 -> nil A = v0 /\ v3 = v4)).
-      simpl; intuition.
-    + eapply (caseS' v1). eapply (caseS' v2).
-      intros h2 t2 h1 t1. simpl. intro H.
-      destruct (cons_inj H). destruct (IHm _ _ H1). subst. intuition.
-  Qed.
-
-  Lemma flip_inv {A} {m} {n} (v1 : Vector.t A (m + n)) (v2 : Vector.t A (n + m)) : 
-    flip v1 = v2 -> v1 = flip v2.
-  Proof.
-    intro. rewrite <- H. clear H v2. unfold flip. apply JMeq_eq.
-    eapply (split_ind v1). intros.
-    eapply (split_ind (append v2 v0)). intros.
-    rewrite H. destruct (vec_append_inj H0). subst. reflexivity.
-  Qed.
-
-  Lemma sum_ext m n R (f g : Rel.T m -> Rel.T n) : 
-    (forall x, f x = g x) -> Rel.sum R f = Rel.sum R g.
-  Proof.
-    intro. apply Rel.p_ext. intro.
-    do 2 rewrite Rel.p_sum. repeat f_equal. extensionality x.
-    destruct (Rel.T_eqb (g x) t) eqn:e; rewrite <- H in e; exact e.
-  Qed.
-
-
-(*
-
-  Lemma tml_sem_cons s G :
-    forall i j j1 j2 h1 h2,
-    Ev.tml_sem (s::G) (concat
-     ((fix aux (l0 : list (list Name)) (i0 : nat) {struct l0} : list (list pretm) :=
-         match l0 with
-         | Datatypes.nil => Datatypes.nil
-         | a :: tl => List.map (fun x : Name => tmvar (i0, x)) a :: aux tl (S i0)
-         end) (s::G) i)) j (Ev.env_app (s::List.nil) G h1 h2) ~=
-    Ev.tml_sem (s::List.nil) (concat
-     ((fix aux (l0 : list (list Name)) (i0 : nat) {struct l0} : list (list pretm) :=
-         match l0 with
-         | Datatypes.nil => Datatypes.nil
-         | a :: tl => List.map (fun x : Name => tmvar (i0, x)) a :: aux tl (S i0)
-         end) (s::List.nil) i)) j1 h1 ++
-    Ev.tml_sem G (concat
-     ((fix aux (l0 : list (list Name)) (i0 : nat) {struct l0} : list (list pretm) :=
-         match l0 with
-         | Datatypes.nil => Datatypes.nil
-         | a :: tl => List.map (fun x : Name => tmvar (i0, x)) a :: aux tl (S i0)
-         end) G i)) j2 h2.
-  Proof.
-    intros. simpl. induction s; simpl; intuition.
-    + admit.
-    + rewrite eq_rect_r_eq_refl. apply eq_JMeq. f_equal.
-      -
-
-  Lemma tml_sem_app G1 :
-    forall G2 j j1 j2 h1 h2,
-    Ev.tml_sem (G1 ++ G2) (tmlist_of_ctx (G1 ++ G2)) j (Ev.env_app _ _ h1 h2) 
-      ~= Ev.tml_sem G1 (tmlist_of_ctx G1) j1 h1 ++ Ev.tml_sem G2 (tmlist_of_ctx G2) j2 h2.
-  Proof.
-    unfold tmlist_of_ctx, mapi. generalize 0 as i.
-    elim G1; simpl; intuition.
-    + destruct h1; simpl in e. simpl. destruct x.
-      - unfold Ev.env_app. simpl. apply Ev.tml_sem_pi.
-        destruct h2. simpl. apply eq_JMeq. f_equal. apply proof_irrelevance.
-      - discriminate e.
-    + simpl.
-
- destruct h2. simpl.
-        apply eq_JMeq. f_equal. generalize dependent j2. generalize dependent j. generalize dependent G2.
-      elim l2; simpl; intuition.
-      repeat rewrite eq_rect_r_eq_refl.
-      apply eq_JMeq. f_equal.
-      admit.
-      apply JMeq_eq. apply H0.
-    + rewrite eq_rect_r_eq_refl. destruct a; simpl; intuition.
-      - destruct l1. 
-
-
-  Lemma tml_sem_app l1 :
-    forall l2 G1 G2 j j1 j2 h1 h2,
-    length l1 = length (concat G1) ->
-    Ev.tml_sem (G1 ++ G2) (l1 ++ l2) j (Ev.env_app _ _ h1 h2) 
-      ~= Ev.tml_sem G1 l1 j1 h1 ++ Ev.tml_sem G2 l2 j2 h2.
-  Proof.
-    elim l1; simpl; intuition.
-    + generalize dependent j2. generalize dependent j. generalize dependent G2.
-      elim l2; simpl; intuition.
-      repeat rewrite eq_rect_r_eq_refl.
-      apply eq_JMeq. f_equal.
-      admit.
-      apply JMeq_eq. apply H0.
-    + rewrite eq_rect_r_eq_refl. destruct a; simpl; intuition.
-      - destruct l1. 
-
-(* makes me wonder if it is even true 
-
-maybe it should be
-
-    Ev.tml_sem (G1 ++ G2) (tmlist_of_ctx (G1 ++ G2)) j (Ev.env_app _ _ h1 h2) 
-      ~= Ev.tml_sem G1 (tmlist_of_ctx G1) j1 h1 ++ Ev.tml_sem G2 (tmlist_of_ctx G2) j2 h2.
-
-but this form is unlikely to be provable directly
-we will probably have to unfold the def of tmlist_of_ctx
-and then generalize wrt the index used in mapi
- *)
-
-unfold Ev.env_app. simpl. 
-      destruct h2.
-      
-
-*)
-
   Fixpoint tmlist_of_ctx_i (G: Ctx) : nat -> list pretm := 
     fun i => match G with
     | List.nil => List.nil
@@ -481,189 +142,12 @@ unfold Ev.env_app. simpl.
     f_equal. apply IHG.
   Qed.
 
-  Lemma tml_sem_app G tml1 tml2 j h :
-    forall j1 j2,
-      Ev.tml_sem G (tml1++tml2) j h = Ev.tml_sem G tml1 j1 h ++ Ev.tml_sem G tml2 j2 h.
-  Proof.
-    induction tml1; simpl; intuition.
-    + apply JMeq_eq. apply Ev.tml_sem_pi. reflexivity.
-    + rewrite eq_rect_r_eq_refl. f_equal.
-      - apply JMeq_eq. apply Ev.tm_sem_pi. reflexivity.
-      - apply IHtml1.
-  Qed.
-
-  Lemma eq_tml_sem :
-    forall G1 G2, G1 = G2 -> forall tml1 tml2, tml1 = tml2 ->
-    forall j1 j2 h1 h2, h1 ~= h2 ->
-    Ev.tml_sem G1 tml1 j1 h1 ~= Ev.tml_sem G2 tml2 j2 h2.
-  Proof.
-    intros G1 G2 eG. rewrite eG.
-    intros tml1 tml2 etml. rewrite etml. intros.
-    apply Ev.tml_sem_pi. exact H.
-  Qed.
-
-  Lemma to_list_append {A} {m} {n} (v1:Vector.t A m) (v2:Vector.t A n) : 
-    to_list (append v1 v2) = to_list v1 ++ to_list v2.
-  Proof.
-    elim v1; simpl; intuition.
-    unfold to_list. f_equal. exact H.
-  Qed.
-
-  Axiom tm_sem_tm_var : forall (P : Value -> Prop) G n a j h,
-    (forall H, P (unopt (Ev.env_lookup G h (n,a)) H)) ->
-    P (Ev.tm_sem G (tmvar (n,a)) j h).
-
-(*
-  Lemma j_tm_sem_tmvar s G1 G2 h: 
-    forall a Stm Hs Has, 
-    Ev.j_tm_sem (G1 ++ s :: G2) (tmvar (length G1, a)) Stm ->
-    Stm h = Ev.var_sem (length G1) a (G1 ++ s :: G2) s Hs Has h.
-  Proof.
-    intros. inversion H. 
-    pose (H4' := existT_projT2_eq _ _ _ H4); clearbody H4'; clear H4.
-    rewrite <- H4'. 
-    enough (s = s0). subst. f_equal. apply proof_irrelevance.
-    apply JMeq_eq. generalize Has0. elim Has; intros.
-    + generalize (eq_refl (a::s)). 
-      dependent inversion Has1 with (fun s1 (Hinv : j_var a s1)  => s1 = a::s -> Hinv ~= j_varhd a s n).
-      - intro. apply eq_JMeq. f_equal. apply proof_irrelevance.
-      - contradiction n0. reflexivity.
-    + generalize (eq_refl (b::s)). 
-      dependent inversion Has1 with (fun s1 (Hinv : j_var a s1)  => s1 = b::s -> Hinv ~= j_varcons a b s n j).
-      - contradiction n.
-      - intro. apply eq_JMeq. f_equal. apply proof_irrelevance. apply JMeq_eq. apply H0.
-    + clear h Stm Has H Has0 H0 H2 H4'. generalize dependent Hs0. elim G1; intros.
-      - injection Hs0. intuition.
-      - apply H. exact Hs0.
-  Qed.
-
-  Lemma p_unopt {A} : 
-    forall (P : A -> Prop) (x : option A) Hx, 
-    (forall y, x = Some y -> P y) -> P (unopt x Hx).
-  Proof.
-    intros. destruct x. apply H. reflexivity. contradiction Hx. reflexivity.
-  Qed.
-*)
-
-  Lemma projT1_env_app G1 G2 h1 h2 : 
-    projT1 (Ev.env_app G1 G2 h1 h2) = projT1 h1 ++ projT1 h2.
-  Proof.
-    admit.
-  Admitted.
-
-  Lemma ev_split_ind {A} {m} {n} (v : Vector.t A (m + n)) :
-    forall (P : forall m n, (Vector.t A m * Vector.t A n) -> Prop),
-    (forall v1 v2, v = append v1 v2 -> P m n (v1,v2)) ->
-    P m n (Ev.split v).
-  Proof.
-    admit.
-  Admitted.
-
-
-  Lemma projT1_env_of_tuple G x : 
-    projT1 (Ev.env_of_tuple G x) = to_list x.
-  Proof.
-    induction G.
-    + simpl in x. eapply (case0 (fun v => List.nil = to_list v) _ x). Unshelve. reflexivity.
-    + simpl. simpl in x. 
-      enough (forall v1 v2, x = append v1 v2 -> 
-        to_list v1 ++ projT1 (Ev.env_of_tuple G v2) = to_list x).
-      erewrite <- (H (fst (Ev.split x)) (snd (Ev.split x))). reflexivity.
-      apply JMeq_eq.
-      apply (ev_split_ind x (fun m n p => x ~= append (fst p) (snd p))).
-      intros. rewrite H0. reflexivity.
-      intros. rewrite H. rewrite to_list_append. f_equal. apply IHG.
-  Qed.
-
-(*
-  Lemma scm_env_combine :
-    forall s G x h y p,
-    Ev.scm_env s (projT1 (Ev.env_app (s :: Datatypes.nil) G (Ev.env_of_tuple (s :: Datatypes.nil) x) h)) = (y,p) ->
-    y = List.combine s (to_list x).
-  Proof.
-    intros. simpl in x. generalize x y H. clear x y H.
-    induction s.
-    + simpl. intros. injection H. intuition.
-    + simpl. intro. 
-      destruct (@Ev.split Rel.V (@length Name s) O
-                         (@tl Rel.V
-                            ((fix add (n m : nat) {struct n} : nat :=
-                                match n return nat with
-                                | O => m
-                                | S p0 => S (add p0 m)
-                                end) (@length Name s) O) x)) eqn:e.
-      simpl. unfold Rel.V. 
-      destruct (Ev.scm_env s (((fix fold_right_fix (n : nat) (v : Vector.t Value n) (b : list Value) {struct v} : 
-        list Value := match v with
-                      | nil _ => b
-                      | cons _ a0 n0 w => a0 :: fold_right_fix n0 w b
-                      end) (length s) t Datatypes.nil ++ Datatypes.nil) ++ projT1 h)) eqn:e0.
-      intros y Hinj; injection Hinj; clear Hinj; intros.
-      rewrite <- H0. rewrite (Vector.eta x). simpl. f_equal. apply IHs.
-      rewrite <- H, <- e0. rewrite projT1_env_app. f_equal. f_equal.
-      rewrite projT1_env_of_tuple. generalize (eq_JMeq e).
-      eapply (ev_split_ind (tl x) (fun m n p => p ~= (t, t0) -> (_ :Prop))).
-      intros. rewrite H1. simpl. rewrite (to_list_append v1 v2).
-      replace (to_list v2) with (@List.nil Value). f_equal.
-      injection (JMeq_eq H2). intros. rewrite H4. reflexivity.
-      eapply (case0 (fun v => List.nil = to_list v) _ v2). Unshelve. reflexivity.
-  Qed.
-
-  Lemma var_sem_env_app s G1 G2 h1 h2: 
-    forall a Hs Has x z1 z2 y p, 
-    Ev.scm_env s (projT1 (Ev.env_app (s :: Datatypes.nil) G2 (Ev.env_of_tuple (s :: Datatypes.nil) x) h2)) = (y,p) ->
-    find (fun x0 => if Db.Name_dec (fst x0) a then true else false) y = Some (z1,z2) ->
-    Ev.var_sem (length G1) a (G1 ++ s :: G2) s Hs Has 
-      (Ev.env_app _ _ h1 (Ev.env_app (s::List.nil) _ (Ev.env_of_tuple _ x) h2))
-    = z2.
-  Proof.
-    intros. unfold Ev.var_sem. apply p_unopt.
-    intro. unfold Ev.env_lookup. apply bind_elim.
-    + intro. rewrite proj1T_env_app. 
-      replace (length G1) with (length G1 + 0). rewrite Ev.nth_error_ctx_env_app_eq.
-      - unfold Ev.ctx_env. rewrite H. simpl.
-        intro. injection H1. clear H1. intro.
-        subst. apply bind_elim.
-        * intro. rewrite H0. intro. injection H1. clear H1. intro. subst.
-          unfold ret. intro. injection H1; clear H1; intro. intuition.
-        * intros. discriminate H2.
-      - simpl. repeat rewrite app_length. rewrite length_to_list. simpl.
-        f_equal. omega. destruct h2. simpl. apply Nat.eqb_eq. exact e.
-      - destruct h1. simpl. apply Nat.eqb_eq. exact e.
-      - omega.
-    + intros. discriminate H2.
-  Qed.
-*)
-
   Derive Inversion j_nil_sem with (forall G Snil, Ev.j_tml_sem0 G List.nil Snil) Sort Prop.
   Derive Inversion j_cons_sem with (forall G hd tl Scons, Ev.j_tml_sem0 G (hd::tl) Scons) Sort Prop.
-
-  Lemma JMeq_cast_eq S T e x y : x ~= y -> cast S T e x = y.
-  Proof.
-    generalize x. rewrite e. simpl. intuition. apply JMeq_eq. exact H.
-  Qed.
-
-  Lemma eq_vector_to_list {A} {m} {n} (v1 : Vector.t A m) (v2 : Vector.t A n) :
-    m = n -> to_list v1 = to_list v2 -> v1 ~= v2.
-  Proof.
-    intro. generalize dependent v1. rewrite H. intro.
-    apply (rect2 (fun {n} w1 w2 => to_list w1 = to_list w2 -> w1 ~= w2)); intuition.
-    unfold to_list in H1; simpl in H1. injection H1.
-    clear H1; intros. rewrite H2.
-    eapply (f_JMeq _ _ (cons A b n0)). apply JMeq_eq. apply H0. exact H1.
-  Qed.
 
   Derive Inversion j_tmvar_sem with (forall G n a Svar, Ev.j_tm_sem0 G (tmvar (n,a)) Svar) Sort Prop.
   Derive Inversion jfv_O_sem with (forall s G a Svar, Ev.j_fvar_sem (s::G) O a Svar) Sort Prop.
   Derive Inversion jfv_S_sem with (forall s G i a Svar, Ev.j_fvar_sem (s::G) (S i) a Svar) Sort Prop.
-
-  Axiom subenv1_app : forall G1 G2 h1 h2, Ev.subenv1 (Ev.env_app G1 G2 h1 h2) = h1.
-  Axiom env_app_nil_l : forall G h1 h2, Ev.env_app List.nil G h1 h2 = h2.
-  Axiom env_hd_hd : forall a s G (h : Ev.env ((a::s)::G)) x, 
-    List.hd_error (projT1 h) = Some x -> Ev.env_hd h = x.
-  Axiom env_tl_tl : forall a s G (h : Ev.env ((a::s)::G)),
-    projT1 (Ev.env_tl h) = List.tl (projT1 h).
-  Axiom tl_append : forall A m n (v1 : Vector.t A (S m)) (v2 : Vector.t A n), tl (append v1 v2) = append (tl v1) v2.
 
   Lemma j_var_sem_tech : forall a s1 s2 (x : Rel.T (S (length s2))) (y : Rel.T (length s1)) e,
     forall Sa,
@@ -676,7 +160,7 @@ unfold Ev.env_app. simpl.
         apply eq_JMeq. apply env_hd_hd.
         rewrite (projT1_env_app ((a::s2)::List.nil) List.nil). simpl.
         rewrite app_nil_r. replace y with (Vector.nil Rel.V). simpl.
-        apply (ev_split_ind (@tl Rel.V
+        apply (split_ind (@tl Rel.V
                 ((fix add (n m : nat) {struct n} : nat := match n with
                                                           | 0 => m
                                                           | S p => S (add p m)
@@ -697,7 +181,7 @@ unfold Ev.env_app. simpl.
         apply eq_JMeq. f_equal. apply Ev.env_eq.
         rewrite env_tl_tl. rewrite (projT1_env_app ((a0::s1++a::s2)::List.nil) List.nil).
         rewrite projT1_env_of_tuple. simpl.
-        apply (ev_split_ind (@tl Rel.V
+        apply (split_ind (@tl Rel.V
                 ((fix add (n m : nat) {struct n} : nat := match n with
                                                           | 0 => m
                                                           | S p => S (add p m)
@@ -722,6 +206,7 @@ unfold Ev.env_app. simpl.
         * rewrite plus_0_r. reflexivity.
   Qed.
 
+  (* XXX: move to Util *)
   Lemma skipn_app_l : forall A (l1 l2: list A) n, n <= length l1 -> skipn n (l1++l2) = skipn n l1 ++ l2.
   Proof.
     intros. generalize dependent n. induction l1.
@@ -751,7 +236,7 @@ unfold Ev.env_app. simpl.
     + simpl in H3. eapply (jfv_S_sem _ _ _ _ _ (fun s0 G0 i0 a0 Svar0 => _) _ H3). Unshelve.
       simpl; intros; subst. rewrite <- (existT_projT2_eq _ _ _ H6); clear H6.
       eapply (JMeq_trans _ (IHG1 _ H4 (@Ev.subenv2 (a0::List.nil) G1 h1))). Unshelve.
-      apply eq_JMeq. f_equal. apply Ev.env_eq. simpl. 
+      apply eq_JMeq. f_equal. apply Ev.env_eq. simpl.
       erewrite skipn_app_l.
       - reflexivity.
       - destruct h1. simpl. rewrite <- (proj1 (Nat.eqb_eq _ _) e0).
@@ -797,7 +282,7 @@ unfold Ev.env_app. simpl.
             apply JMeq_eq. eapply (f_JMequal (@to_list Rel.V _) (@to_list Rel.V _)). Unshelve.
             -- eapply (f_JMeq _ _ (@to_list Rel.V)). repeat rewrite app_length. simpl. omega.
             -- symmetry. apply cast_JMeq. 
-               apply (ev_split_ind (cast (Vector.t Rel.V (length s1 + S (length s2))) (Rel.T (length (s1 ++ a :: s2) + 0)) e (append y x))).
+               apply (split_ind (cast (Vector.t Rel.V (length s1 + S (length s2))) (Rel.T (length (s1 ++ a :: s2) + 0)) e (append y x))).
                intros. simpl. enough (v2 = Vector.nil _). enough (append y x ~= v1).
               ** apply eq_vector_to_list. repeat rewrite app_length; simpl; omega.
                 transitivity (to_list (append (append y (cons _ (hd x) 0 (nil _))) (tl x))).
@@ -832,67 +317,6 @@ unfold Ev.env_app. simpl.
             -- repeat rewrite app_length. simpl. rewrite plus_0_r. rewrite <- plus_assoc. reflexivity.
       - rewrite <- Vector.eta. reflexivity.
   Qed.
-
-(*
-  Lemma f_JMequal_pi {A : Prop} {B : A -> Type} {A' : Prop} {B' : A' -> Type} 
-    {ea : A = A'} {eb : B ~= B'} :
-    forall (f : forall a, B a) (g : forall a', B' a') x y, f ~= g -> f x ~= g y.
-
-          eapply (@JMeq_trans _ x0 x1 _ (Stml0 (Ev.env_app _ _ h1 (Ev.env_app ((s1++a::s2)::List.nil) G2 
-        (Ev.env_of_tuple ((s1++a::s2)::List.nil) (cast _ _ e (Vector.append y x))) h2)))).
-          ++ apply eq_JMeq. f_equal.
-          ++ erewrite <- (IHs2 (s1++(a::List.nil)) _ _ (tl x) _ _ h1 h2). (* Stml0' H4' (y++[hd x])' e' *)
-
-(* mi sa che tocca affiancare a x anche y... *)
-
- (* apply IHl. *) admit.
-      - symmetry. apply eq_JMeq. apply Vector.eta.
-  Admitted.
-      
-      rewrite (Vector.eta x).
-
-      cut (forall Shd Stl, Ev.j_tm_sem (G1++s::G2) (tmvar (length G1,a)) Shd ->
-        Ev.j_tml_sem (G1++s::G2) (List.map (fun x1 => tmvar (length G1,x1)) l) Stl ->
-        Stml ~= fun h => Vector.cons _ (Shd h) _ (Stl h)).
-      intro.
-
-cut (Stml ~= fun h => Vector.nil _).
-      - intro HS. rewrite HS. eapply (case0 (fun v => nil Rel.V ~= v) _ x). Unshelve. reflexivity.
-      - apply JMeq_eq. eapply (j_nil_sem _ _ (fun tml0 Stml0 => Stml0 ~= _) _ H). Unshelve.
-        intros. simpl. rewrite <- (existT_projT2_eq _ _ _ H1). reflexivity.
-    +
-        simple inversion H. with 
-          (fun tml0 Stml0 => Stml0 ~= (fun _ : Ev.env (G1 ++ Datatypes.nil :: G2) => nil Rel.V)).
-
-    intros x Stml e H. unfold Ev.j_tml_sem in H.
-    enough (forall tml0 Stml0, 
-      Ev.j_tml_sem0 (G1++s::G2) tml0 Stml0 ->
-      tml0 = List.map (fun x1 => tmvar (length G1,x1)) s ->
-      forall h1 h2, Stml0 (Ev.env_app _ ((s::List.nil)++G2) h1 
-        (Ev.env_app _ G2 (Ev.env_of_tuple (s::List.nil) (cast _ _ e x)) h2)) ~= x).
-    apply H0. exact H. reflexivity.
-    intros tml0 Stml0 H'. induction H'.
-    + destruct s; simpl; intros.
-      - eapply (case0 (fun v => nil Rel.V ~= v) _ x).
-      - discriminate H0.
-    +
-
-
-    induction H. with (fun G0 tml0 Stml0 => G1 ++ s :: G2 = G0 -> _).
-      forall 
-  Qed.
-
-
-  Lemma j_tml_sem_env_app_subind s2 G1 G2 : 
-    forall s1 Stml,
-    Ev.j_tml_sem (G1 ++ (s1 ++ s2) :: G2) (List.map (fun x1 => tmvar (length G1, x1)) s2) Stml ->
-    forall (x : Rel.T (length s2)) (y : Rel.T (length s1)) e,
-    forall h1 h2, Stml (Ev.env_app _ _ h1 (Ev.env_app ((s1++s2)::List.nil) G2 
-        (Ev.env_of_tuple ((s1++s2)::List.nil) (cast _ _ e (Vector.append y x))) h2)) 
-        ~= x.
-
-
-*)
 
   Lemma j_tml_sem_env_app s G1 G2 :
     forall Stml,
@@ -1069,8 +493,8 @@ cut (Stml ~= fun h => Vector.nil _).
             Focus 2. do 2 rewrite length_tmlist_of_ctx_i. rewrite <- app_assoc. reflexivity.
           apply  Ev.env_JMeq. rewrite <- app_assoc. reflexivity.
           rewrite projT1_env_app. rewrite projT1_env_app. rewrite projT1_env_app. rewrite projT1_env_app.
-          rewrite (@projT1_env_app (a::G) G2). rewrite (@projT1_env_app (a::List.nil) G). 
-          rewrite projT1_env_of_tuple. rewrite projT1_env_of_tuple. rewrite projT1_env_of_tuple.
+          rewrite (@projT1_env_app (a::G) G2). rewrite (@projT1_env_app (a::List.nil) G).
+          rewrite projT1_env_of_tuple. rewrite projT1_env_of_tuple.
           simpl. rewrite <- app_assoc. rewrite <- app_assoc. f_equal. f_equal.
           apply JMeq_eq. eapply (f_JMequal to_list to_list). Unshelve.
           ++ rewrite plus_0_r. reflexivity.
@@ -1078,137 +502,6 @@ cut (Stml ~= fun h => Vector.nil _).
           ++ rewrite plus_0_r. reflexivity.
           ++ rewrite plus_0_r. reflexivity.
     Qed.
-
-(*
-  Lemma tml_sem_env_app_subind s G1 G2 h1 h2:
-    forall s0 j (x : Rel.T (length s)) (y : Rel.T (length s0)) e,
-    Ev.tml_sem (G1 ++ ((s0 ++ s) :: G2)) (List.map (fun x1 => tmvar (length G1, x1)) s) j
-      (Ev.env_app _ _ h1 (Ev.env_app ((s0++s)::List.nil) G2 
-        (Ev.env_of_tuple _ (cast _ _ e (Vector.append y x))) h2))
-    = to_list x.
-  Proof.
-    elim s; simpl; intuition.
-    + rewrite eq_rect_r_eq_refl. apply (Vector.case0 (fun x => List.nil = to_list x)). reflexivity.
-    + rewrite eq_rect_r_eq_refl.
-      replace (to_list x) with (hd x::to_list (tl x)). f_equal.
-      - apply tm_sem_tm_var. intro.
-
-(* add lemma on semantics (tm_sem) of tm_var *) admit.
-      - enough (Rel.T (length s0 + 1) = Rel.T (length (s0 ++ a :: Datatypes.nil))).
-        enough (Rel.T (length (s0++a::List.nil) + length l) = Rel.T (length ((s0++a::List.nil) ++ l) + 0)).
-        enough (j0 : j_tml (G1 ++ ((s0 ++ a :: Datatypes.nil) ++ l) :: G2) (List.map (fun x1 : Name => tmvar (length G1, x1)) l)).
-        rewrite <- (H (s0++(a::List.nil)) j0 (tl x) 
-          (cast _ _ H0 (Vector.append y (Vector.cons _ (hd x) _ (Vector.nil _)))) H1).
-        apply JMeq_eq. apply eq_tml_sem; auto.
-        * rewrite <- app_assoc. reflexivity.
-        * (* various equational lemmas on equality of env_app *) admit.
-        * rewrite <- app_assoc. intro. intro. apply j. right. exact H2.
-        * f_equal. rewrite <- app_assoc. repeat rewrite app_length. omega.
-        * rewrite app_length. reflexivity.
-      - rewrite (Vector.eta x). reflexivity.
-  Admitted.
-
-
-  Lemma tml_sem_env_app G :
-    forall G1 G2 j x h1 h2,
-    Ev.tml_sem (G1 ++ G ++ G2) (tmlist_of_ctx_i G (length G1)) j 
-      (Ev.env_app G1 (G ++ G2) h1 (Ev.env_app G G2 (Ev.env_of_tuple G x) h2)) ~= to_list x.
-  Proof.
-    induction G; simpl; intuition.
-    + rewrite eq_rect_r_eq_refl. apply (Vector.case0 (fun x => List.nil ~= to_list x)). reflexivity.
-    + cut (j_tml ((G1 ++ (a::List.nil)) ++ G ++ G2)
-            (List.map (fun x0 : Name => tmvar (length G1, x0)) a 
-            ++ tmlist_of_ctx_i G (length (G1++(a::List.nil))))).
-      - intro j0.
-        cut (exists e, Ev.tml_sem _ _ j0 (Ev.env_app _ _ 
-          (Ev.env_app _ _ h1 (Ev.env_of_tuple (a::List.nil) (cast _ _ e (fst (split x)))))
-          (Ev.env_app _ _ (Ev.env_of_tuple G (snd (split x))) h2)) ~= to_list x).
-        * intro H; destruct H. eapply (JMeq_trans _ H). Unshelve. apply eq_tml_sem.
-          ++ rewrite <- app_assoc. reflexivity.
-          ++ rewrite app_length. rewrite plus_comm. reflexivity.
-          ++ (* eq lemmas on env_app *) admit.
-        * cut (Vector.t Rel.V (length a) = Rel.T (list_sum (List.map (length (A:=Name)) (a::List.nil)))).
-          ++ intro e. exists e.
-            enough (j1 : j_tml ((G1 ++ a :: List.nil) ++ G ++ G2) (List.map (fun x0 => tmvar (length G1, x0)) a)).
-            enough (j2 : j_tml ((G1 ++ a :: List.nil) ++ G ++ G2) (tmlist_of_ctx_i G (length (G1++a::List.nil)))).
-            rewrite (tml_sem_app _ _ _ _ _ j1 j2).
-            replace (to_list x) with (to_list (fst (split x)) ++ to_list (snd (split x))).
-            apply eq_JMeq. f_equal.
-            -- generalize (fst (split x)). intro x0.
-              enough (j3 : j_tml (G1 ++ (Datatypes.nil ++ a) :: G ++ G2) (List.map (fun x1 : Name => tmvar (length G1, x1)) a)).
-              enough (Rel.T (@length Rel.V Datatypes.nil + length a) = 
-                Rel.T (list_sum (List.map (length (A:=Name)) ((List.nil++a)::List.nil)))).
-              rewrite <- (tml_sem_env_app_subind a G1 (G++G2) 
-                h1 (Ev.env_app _ _ (Ev.env_of_tuple G (snd (split x))) h2) List.nil j3 x0 (Vector.nil _) H).
-              ** apply JMeq_eq. apply eq_tml_sem; auto.
-                +++ rewrite <- app_assoc. reflexivity.
-                +++ (* eq lemmas on env_app *) admit.
-              ** simpl. f_equal. omega.
-              ** intro. intro. apply j. apply List.in_or_app. left. exact H.
-            -- apply JMeq_eq. apply IHG.
-            -- replace x with (Vector.append (fst (split x)) (snd (split x))) at 3. 
-              apply split_ind. intros. symmetry. apply to_list_append.
-              apply JMeq_eq.
-              apply (split_ind x (fun _ _ v => append (fst v) (snd v) ~= x)). intros.
-              rewrite H. reflexivity.
-            -- intro. intro. rewrite <- app_assoc. simpl. apply j. apply in_or_app. right. 
-              rewrite app_length in H. simpl in H. rewrite plus_comm in H. exact H.
-            -- intro. intro. rewrite <- app_assoc. simpl. apply j. apply in_or_app. left. exact H.
-          ++ simpl. rewrite plus_comm. reflexivity.
-      - rewrite <- app_assoc. rewrite app_length. simpl. rewrite plus_comm. exact j.
-  Admitted.
-
-  Lemma v_tml_sem_env_app G G1 j x h :
-    Ev.v_tml_sem (G1 ++ G) (tmlist_of_ctx G1) j (Ev.env_app G1 G (Ev.env_of_tuple G1 x) h) ~= x.
-  Proof.
-    unfold Ev.v_tml_sem. apply JMeq_eq_rect.
-    + unfold tmlist_of_ctx. rewrite length_concat_list_sum.
-      f_equal. f_equal. unfold mapi. generalize 0. elim G1; simpl; intuition.
-      f_equal. rewrite map_length. reflexivity.
-      rewrite H. reflexivity.
-    + apply (@JMeq_trans _ _ _ _ (of_list (to_list x))).
-      - eapply (f_JMequal of_list of_list _ _ JMeq_refl). Unshelve. 
-        generalize dependent j. rewrite tmlist_of_ctx_O. intro. 
-        enough (h0 : Ev.env List.nil).
-        replace (Ev.env_app G1 G (Ev.env_of_tuple G1 x) h)
-          with (Ev.env_app _ _ h0 (Ev.env_app G1 G (Ev.env_of_tuple G1 x) h)).
-        apply (tml_sem_env_app G1 List.nil G j x).
-        destruct h0. unfold Ev.env_app. simpl. apply JMeq_eq.
-        enough (Hx0 : x0 = @List.nil (list Rel.V)).
-        eapply (f_JMequal_pi
-          (existT (fun h0 : Ev.preenv => List.map (length (A:=Name)) (G1 ++ G) = List.map (length (A:=Value)) h0)
-            (x0 ++ projT1 (Ev.env_of_tuple G1 x) ++ projT1 h))
-          (existT (fun h0 : Ev.preenv => List.map (length (A:=Name)) (G1 ++ G) = List.map (length (A:=Value)) h0)
-            (projT1 (Ev.env_of_tuple G1 x) ++ projT1 h))).
-        eapply (f_JMequal
-          (existT (fun h0 : Ev.preenv => List.map (length (A:=Name)) (G1 ++ G) = List.map (length (A:=Value)) h0))
-          (existT (fun h0 : Ev.preenv => List.map (length (A:=Name)) (G1 ++ G) = List.map (length (A:=Value)) h0))).
-        Unshelve.
-        reflexivity.
-        rewrite Hx0; reflexivity.
-        destruct x0; auto; discriminate e.
-        exists List.nil. reflexivity. 
-        reflexivity.
-        reflexivity.
-        rewrite Hx0; reflexivity.
-        rewrite Hx0; reflexivity.
-        reflexivity.
-        reflexivity.
-      - elim x; simpl; intuition.
-        change cons with VectorDef.cons.
-        cut (VectorDef.cons Rel.V h0 ~= VectorDef.cons Rel.V h0). intro.
-        cut (VectorDef.cons Rel.V h0 (length (to_list t)) ~= VectorDef.cons Rel.V h0 n). intro.
-        eapply (f_JMequal _ _ _ _ H1). Unshelve.
-        exact H.
-        eapply (f_JMequal _ _ _ _ H0). Unshelve.
-        apply eq_JMeq. apply length_to_list. 
-        reflexivity.
-        rewrite length_to_list. reflexivity.
-        rewrite length_to_list. reflexivity.
-        reflexivity.
-        reflexivity.
-  Qed.
-*)
 
   Lemma eq_memb_dep_elim1 : forall (P : nat -> Prop) m n (S1:Rel.R m) (S2 : Rel.R n) r2,
     m = n -> S1 ~= S2 ->
@@ -1236,58 +529,100 @@ cut (Stml ~= fun h => Vector.nil _).
     intros; subst. rewrite <- H1. apply H2. reflexivity.
   Qed.
 
+  Lemma filter_supp_eq_tech n (al : list (Rel.T n)) x (Hal : NoDup al) :
+    (List.In x al -> filter (fun x0 => Rel.T_eqb x0 x) al = x::List.nil)
+    /\ (~List.In x al -> filter (fun x0 => Rel.T_eqb x0 x) al = List.nil).
+  Proof.
+    induction Hal.
+    + split; intro.
+      contradiction H. reflexivity.
+    + destruct IHHal. split; intro.
+      - inversion H2. simpl. replace (Rel.T_eqb x0 x) with true.
+        rewrite H3. f_equal. apply H1. rewrite <- H3. exact H.
+        symmetry. apply Rel.T_eqb_eq. exact H3.
+        simpl. replace (Rel.T_eqb x0 x) with false. apply H0. exact H3.
+        destruct (Rel.T_eqb x0 x) eqn:e; intuition. replace x with x0 in H3. contradiction H.
+        apply Rel.T_eqb_eq. exact e.
+      - simpl. replace (Rel.T_eqb x0 x) with false. apply H1. intro. apply H2. right. exact H3.
+        destruct (Rel.T_eqb x0 x) eqn:e; intuition. replace x with x0 in H2. contradiction H2. left. reflexivity.
+        apply Rel.T_eqb_eq. exact e.
+  Qed.
+
   Lemma filter_supp_elim n R r (P : list (Rel.T n) -> Prop) :
     (List.In r (Rel.supp R) -> P (r::List.nil)) ->
     (~ List.In r (Rel.supp R) -> P List.nil) ->
     P (filter (fun (x0 : Rel.T n) => Rel.T_eqb x0 r) (Rel.supp R)).
   Proof.
-    admit.
-  Admitted.
+    destruct (filter_supp_eq_tech _ (Rel.supp R) r (Rel.p_nodup _ R)).
+    destruct (List.in_dec (Rel.T_dec _) r (Rel.supp R)); intros.
+    rewrite H. apply H1. exact i. exact i.
+    rewrite H0. apply H2. exact n0. exact n0.
+  Qed.
 
   Lemma filter_supp_elim' m n R r (P : list (Rel.T (m+n)) -> Prop) :
     (List.In (flip r) (Rel.supp R) -> P (flip r::List.nil)) ->
     (~ List.In (flip r) (Rel.supp R) -> P List.nil) ->
     P (filter (fun x0 => Rel.T_eqb (flip x0) r) (Rel.supp R)).
   Proof.
-    admit.
-  Admitted.
+    replace (fun x0 => Rel.T_eqb (flip x0) r) with (fun x0 => Rel.T_eqb x0 (flip r)). apply filter_supp_elim. 
+    extensionality x0. apply eq_T_eqb_iff. split; intro.
+    + symmetry. apply flip_inv. symmetry. exact H.
+    + apply flip_inv. exact H.
+  Qed.
+
+  Lemma j_btb_sem_ctx d G Gout T1 s1 T2 s2 Sbtb : 
+    SQLSem3.j_btb_sem d G Gout ((T1, s1) :: (T2, s2) :: Datatypes.nil) Sbtb ->
+    Gout = s1::s2::List.nil.
+  Proof.
+    intro. inversion H. subst.
+    apply (existT_eq_elim H7); clear H7; intros _ H7.
+    apply (existT_eq_elim (JMeq_eq H7)); clear H7; intros _ HSbtb.
+    inversion H8. subst.
+    apply (existT_eq_elim H11); clear H11; intros _ H11.
+    apply (existT_eq_elim (JMeq_eq H11)); clear H11; intros _ HSbtb0.
+    eapply (j_nil_btb_sem _ _ _ _ _ _ H12). Unshelve. intros. subst. reflexivity.
+  Qed.
 
   Lemma j_commutative_join d G T1 T2 s1 s2 sa sb S1 S2 h :
+    length sb = length s1 + length s2 ->
     SQLSem3.j_q_sem d G sa (SELECT * FROM ((T1,s1)::(T2,s2)::List.nil) WHERE TRUE) S1 ->
     SQLSem3.j_q_sem d G sb
       (SELECT (btm_of_tml (tml_of_scm s1 1 ++ tml_of_scm s2 0) sb) FROM ((T2,s2)::(T1,s1)::List.nil) WHERE TRUE)
       S2 ->
     forall ra rb, ra ~= rb -> Rel.memb (S1 h) ra = Rel.memb (S2 h) rb.
   Proof.
-    intros. inversion H. subst. 
+    intros Hlen H H0 ra rb H1. inversion H. subst. 
     apply (existT_eq_elim H9); clear H9; intros _ H9.
     apply (existT_eq_elim (JMeq_eq H9)); clear H9; intros _ HS1.
     inversion H0. subst.
     apply (existT_eq_elim H14); clear H14; intros _ H14.
     apply (existT_eq_elim (JMeq_eq H14)); clear H14; intros _ HS2.
     subst.
-    assert (e' : Rel.T (length (concat G1)) = Rel.T (length (tmlist_of_ctx G1))). admit. (* simple *)
+    assert (HG2 : G2 = s2::s1::List.nil). eapply (j_btb_sem_ctx _ _ _ _ _ _ _ _ H9).
+    assert (e' : Rel.T (length (concat G1)) = Rel.T (length (tmlist_of_ctx G1))). 
+      rewrite Ev.length_tmlist, length_concat_list_sum. reflexivity.
     transitivity (Rel.memb (Rel.sum (Rel.sel (Sbtb h)
         (fun Vl : Rel.T (list_sum (List.map (length (A:=Name)) G1)) =>
             S3.is_btrue (Sc (Ev.env_app G1 G (Ev.env_of_tuple G1 Vl) h))))
       (fun Vl : Rel.T (list_sum (List.map (length (A:=Name)) G1)) =>
          Stml (Ev.env_app G1 G (Ev.env_of_tuple G1 Vl) h))) (cast _ _ e' ra)).
-      apply eq_memb_dep. admit (* simple *).
+      apply eq_memb_dep. rewrite Ev.length_tmlist. reflexivity.
       apply cast_JMeq. reflexivity.
       symmetry. apply cast_JMeq. reflexivity.
       assert (eS2 : (fun _ : Ev.env G =>
         Rel.R (length (List.map snd (btm_of_tml (tml_of_scm s1 1 ++ tml_of_scm s2 0) (List.map snd tml))))) 
-        ~= (fun _ : Ev.env G => Rel.R (length (List.map snd tml)))). admit. (* simple *)
+        ~= (fun _ : Ev.env G => Rel.R (length (List.map snd tml)))). rewrite H13. reflexivity.
       pose (HS2' := @f_JMequal _ _ _ _ eq_refl eS2 _ _ h h HS2 JMeq_refl). clearbody HS2'. simpl in HS2'.
     assert (e'' : Rel.T (length (List.map snd tml)) 
-      = Rel.T (length (List.map fst (btm_of_tml (tml_of_scm s1 1 ++ tml_of_scm s2 0) (List.map snd tml))))). admit. (* simple *)
+      = Rel.T (length (List.map fst (btm_of_tml (tml_of_scm s1 1 ++ tml_of_scm s2 0) (List.map snd tml))))). 
+      rewrite H3, List.map_length in Hlen. do 2 rewrite List.map_length. rewrite Hlen, H3, Hlen. reflexivity.
     transitivity (Rel.memb (Rel.sum
             (Rel.sel (Sbtb0 h)
                (fun Vl : Rel.T (list_sum (List.map (length (A:=Name)) G2)) =>
                 S3.is_btrue (Sc0 (Ev.env_app G2 G (Ev.env_of_tuple G2 Vl) h))))
             (fun Vl : Rel.T (list_sum (List.map (length (A:=Name)) G2)) =>
              Stml1 (Ev.env_app G2 G (Ev.env_of_tuple G2 Vl) h))) (cast _ _ e'' rb)).
-      Focus 2. apply eq_memb_dep. admit (* simple *).
+      Focus 2. apply eq_memb_dep. rewrite <- H3. do 2 rewrite List.map_length. reflexivity.
       eapply (JMeq_trans _ HS2'). Unshelve.
       apply cast_JMeq. reflexivity.
       symmetry. apply cast_JMeq. reflexivity.
@@ -1311,24 +646,32 @@ cut (Stml ~= fun h => Vector.nil _).
     intros. assert (Hr1 : r1 ~= ra). apply (JMeq_trans H). apply cast_JMeq. reflexivity. clear H.
     (* simplify rhs *)
     apply (cast_elim (Rel.T (length s1 + length s2)) rb).
-      (* hopefully simple *) admit.
+      f_equal. exact Hlen.
       intros r2 Hr2.
     apply (cast_elim (Rel.R (length s2 + length s1)) (Sbtb0 h)).
-      (* hopefully simple *) admit.
+      rewrite HG2. simpl. f_equal. omega.
       intros R2 HR2.
     transitivity (Rel.memb (Rel.sum R2 flip) r2).
       Focus 2. apply eq_memb_dep.
-      (* hopefully simple *) admit.
+      rewrite <- H3, <- Hlen. do 2 rewrite List.map_length. reflexivity.
       apply sum_ext_dep.
-      (* hopefully simple *) admit.
-      (* hopefully simple *) admit.
+      rewrite HG2. simpl. omega.
+      rewrite <- H3, <- Hlen. do 2 rewrite List.map_length. reflexivity.
       symmetry. exact HR2.
       intros. symmetry. 
       apply (cast_elim (Ev.env (s2::s1::G) -> Rel.T (length (tml_of_scm s1 1 ++ tml_of_scm s2 0))) Stml1).
-        admit. (* lemmatize *)
+        rewrite List.app_length. unfold tml_of_scm. repeat rewrite List.map_length. 
+        unfold tml_of_scm in H3. rewrite <- H3. rewrite <- Hlen. rewrite List.map_length.
+        rewrite HG2. reflexivity.
       intros Stml1' HStml1'.
       apply (cast_elim (Ev.j_tml_sem (s2::s1::G) (tml_of_scm s1 1 ++ tml_of_scm s2 0) Stml1') H16).
-        admit. (* lemmatize *)
+        unfold btm_of_tml. apply JMeq_eq. 
+        eapply (@f_JMequal _ (fun _ => Type) _ (fun _ => Type) _ _ 
+                 (Ev.j_tml_sem (G2++G) (List.map fst (combine (tml_of_scm s1 1 ++ tml_of_scm s2 0) (List.map snd tml))))
+                 (Ev.j_tml_sem (s2::s1::G) (tml_of_scm s1 1 ++ tml_of_scm s2 0)) _ _ _ HStml1'). Unshelve.
+        Focus 3. rewrite HG2. simpl. rewrite H3. rewrite List.map_length.
+        rewrite H13. erewrite length_combine. reflexivity.
+        unfold tml_of_scm. rewrite List.app_length. do 2 rewrite List.map_length. symmetry. exact Hlen.
       intros H16' _. 
       eapply (JMeq_trans _ (j_tml_sem_flip _ _ _ _ H16' _ _ _ _)). Unshelve.
       + symmetry. apply cast_JMeq. exact Hr2.
@@ -1336,25 +679,68 @@ cut (Stml ~= fun h => Vector.nil _).
         apply (filter_supp_elim _ (Sbtb h) r1); intro;
         apply (filter_supp_elim' _ _ R2 r2 (fun l => _ = list_sum (List.map _ l))); intro; simpl.
         - f_equal. apply (cast_elim (Rel.T (list_sum (List.map (@length _) G2))) (flip r2)).
-          (* rewrite <- length_concat_list_sum. -- from H9 *) admit.
+          rewrite HG2. simpl. unfold Rel.T. f_equal. omega.
           intros fr2 Hfr2. 
           eapply (eq_trans (j_commutative_join_btb _ _ _ _ _ _ _ _ _ _ _ _ 
             fr2 (fst (split r2)) (snd (split r2)) _ _ H8 H9)). Unshelve.
           apply eq_memb_dep.
-          (* from H9 *) admit. exact HR2. symmetry. exact Hfr2.
+          rewrite HG2. simpl. omega.
+          exact HR2. symmetry. exact Hfr2.
           apply (split_ind r2 (fun m n p => r1 ~= append (fst p) (snd p))). intros. simpl.
           rewrite <- H2. apply (JMeq_trans Hr1). apply (JMeq_trans H1). exact Hr2.
           rewrite <- Hfr2. unfold flip.
           apply (split_ind r2 (fun m n p => (let (v1,v2) := p in append v2 v1) ~= append (snd p) (fst p))). 
           intros. simpl. reflexivity.
-        - (* contradiction H+H0 (using H8 H9) *) admit.
-        - (* contradiction H+H0 (using H8 H9) *) admit.
+        - enough (Rel.memb (Sbtb h) r1 > 0).
+          replace (Rel.memb (Sbtb h) r1) with (Rel.memb R2 (flip r2)) in H2.
+          exfalso. apply H0. apply Rel.p_fs. exact H2.
+          enough (exists (rc : Rel.T (length s1)) (rd : Rel.T (length s2)), r2 ~= append rc rd /\ flip r2 ~= append rd rc).
+          decompose record H4. rewrite H7.
+          enough (Rel.T (length s2 + length s1) = Rel.T (list_sum (List.map (length (A:=Name)) G2))).
+          transitivity (Rel.memb (Sbtb0 h) (cast _ _ H6 (append x0 x))).
+          apply eq_memb_dep. rewrite HG2. simpl. omega.
+          symmetry. exact HR2. symmetry. apply cast_JMeq. reflexivity.
+          eapply (j_commutative_join_btb _ _ _ _ _ _ _ _ _ _ _ _ _ _ _ _ _ H9 H8). Unshelve.
+          rewrite HG2. f_equal. simpl. omega.
+          unfold flip. 
+          apply (split_ind r2 (fun m n p => exists rc rd, r2 ~= append rc rd /\ (let (v1,v2) := p in append v2 v1) ~= append rd rc)).
+          intros. exists v1. exists v2. split; apply eq_JMeq; intuition.
+          apply (Rel.p_fs_r _ _ _ H). Focus 3. apply cast_JMeq. reflexivity.
+          apply (JMeq_trans Hr1). apply (JMeq_trans H1). apply (JMeq_trans Hr2). exact H5.
+        - enough (Rel.memb R2 (flip r2) > 0).
+          replace (Rel.memb R2 (flip r2)) with (Rel.memb (Sbtb h) r1) in H2.
+          exfalso. apply H. apply Rel.p_fs. exact H2. 
+          symmetry.
+          enough (exists (rc : Rel.T (length s1)) (rd : Rel.T (length s2)), r2 ~= append rc rd /\ flip r2 ~= append rd rc).
+          decompose record H4. rewrite H7.
+          enough (Rel.T (length s2 + length s1) = Rel.T (list_sum (List.map (length (A:=Name)) G2))).
+          transitivity (Rel.memb (Sbtb0 h) (cast _ _ H6 (append x0 x))).
+          apply eq_memb_dep. rewrite HG2. simpl. omega.
+          symmetry. exact HR2. symmetry. apply cast_JMeq. reflexivity.
+          eapply (j_commutative_join_btb _ _ _ _ _ _ _ _ _ _ _ _ _ _ _ _ _ H9 H8). Unshelve.
+          f_equal. rewrite HG2. simpl. omega.
+          unfold flip. 
+          apply (split_ind r2 (fun m n p => exists rc rd, r2 ~= append rc rd /\ (let (v1,v2) := p in append v2 v1) ~= append rd rc)).
+          intros. exists v1. exists v2. split; apply eq_JMeq; intuition.
+          apply (Rel.p_fs_r _ _ _ H0). Focus 3. apply cast_JMeq. reflexivity.
+          apply (JMeq_trans Hr1). apply (JMeq_trans H1). apply (JMeq_trans Hr2). exact H5.
         - reflexivity.
-      + eapply (f_JMequal Stml1 Stml1'). Unshelve.
-        exact HStml1'. admit. admit. admit.
-      + simpl. rewrite plus_0_r. exact x.
-      + exact h.
-      + simpl. rewrite (Nat.add_0_r (length s1)). reflexivity.
-  Admitted.
+      + rewrite HG2. simpl. rewrite List.map_length. erewrite length_combine. reflexivity.
+        rewrite List.app_length. unfold tml_of_scm. do 2 rewrite List.map_length. symmetry. exact Hlen.
+      + rewrite HG2. simpl. erewrite map_fst_combine. reflexivity. 
+        rewrite List.app_length. unfold tml_of_scm. do 2 rewrite List.map_length. symmetry. exact Hlen.
+      + enough (forall (eG2: Rel.T (list_sum (List.map (length (A:=Name)) G2)) = 
+                             Rel.T (list_sum (List.map (length (A:=Name)) (s2::s1::List.nil)))), 
+          Stml1 (Ev.env_app G2 G (Ev.env_of_tuple G2 y) h) ~=
+          Stml1' (Ev.env_app (s2 :: s1 :: Datatypes.nil) G 
+            (Ev.env_of_tuple (s2 :: s1 :: Datatypes.nil) (cast _ _ eG2 y)) h)).
+        apply H0. generalize dependent y. generalize dependent Stml1. rewrite HG2.
+        intros. eapply (f_JMequal Stml1 Stml1'). Unshelve. exact HStml1'.
+        apply eq_JMeq. f_equal. f_equal. symmetry. apply JMeq_eq. apply cast_JMeq. reflexivity.
+        rewrite HG2. reflexivity. reflexivity.
+        simpl. unfold btm_of_tml. rewrite map_fst_combine. reflexivity.
+        rewrite app_length. unfold tml_of_scm. do 2 rewrite List.map_length. symmetry. exact Hlen.
+      + apply cast_JMeq. symmetry. exact H.
+  Qed.
 
 End RewriteRules.
